p<sub>i</sub> + v<sub>i</sub> · t = p<sub>rock</sub> + v<sub>rock</sub> · t

=> v<sub>i</sub> · t = p<sub>rock</sub> - p<sub>i</sub> + v<sub>rock</sub> · t

=> v<sub>i</sub> · t - v<sub>rock</sub> · t = p<sub>rock</sub> - p<sub>i</sub> + v<sub>rock</sub> · t - v<sub>rock</sub> · t

=> v<sub>i</sub> · t - v<sub>rock</sub> · t = p<sub>rock</sub> - p<sub>i</sub>

=> (v<sub>i</sub> - v<sub>rock</sub>) · t = p<sub>rock</sub> - p<sub>i</sub>

=> t = (p<sub>rock</sub> - p<sub>i</sub>) / (v<sub>i</sub> - v<sub>rock</sub>)



(p<sub>rock<sub>x</sub></sub> - p<sub>i<sub>x</sub></sub>) / (v<sub>i<sub>x</sub></sub> - v<sub>rock<sub>x</sub></sub>) = (p<sub>rock<sub>y</sub></sub> - p<sub>i<sub>y</sub></sub>) / (v<sub>i<sub>y</sub></sub> - v<sub>rock<sub>y</sub></sub>) = (p<sub>rock<sub>z</sub></sub> - p<sub>i<sub>z</sub></sub>) / (v<sub>i<sub>z</sub></sub> - v<sub>rock<sub>z</sub></sub>)





(p<sub>rock<sub>x</sub></sub> - p<sub>i<sub>x</sub></sub>) · (v<sub>i<sub>y</sub></sub> - v<sub>rock<sub>y</sub></sub>) = (p<sub>rock<sub>y</sub></sub> - p<sub>i<sub>y</sub></sub>) · (v<sub>i<sub>x</sub></sub> - v<sub>rock<sub>x</sub></sub>)

<=> (p<sub>rock<sub>x</sub></sub> - p<sub>i<sub>x</sub></sub>) · (v<sub>i<sub>y</sub></sub> - v<sub>rock<sub>y</sub></sub>) - (p<sub>rock<sub>y</sub></sub> - p<sub>i<sub>y</sub></sub>) · (v<sub>i<sub>x</sub></sub> - v<sub>rock<sub>x</sub></sub>) = 0


(p<sub>rock<sub>y</sub></sub> - p<sub>i<sub>y</sub></sub>) · (v<sub>i<sub>z</sub></sub> - v<sub>rock<sub>z</sub></sub>) = (p<sub>rock<sub>z</sub></sub> - p<sub>i<sub>z</sub></sub>) · (v<sub>i<sub>y</sub></sub> - v<sub>rock<sub>y</sub></sub>)

<=> (p<sub>rock<sub>y</sub></sub> - p<sub>i<sub>y</sub></sub>) · (v<sub>i<sub>z</sub></sub> - v<sub>rock<sub>z</sub></sub>) - (p<sub>rock<sub>z</sub></sub> - p<sub>i<sub>z</sub></sub>) · (v<sub>i<sub>y</sub></sub> - v<sub>rock<sub>y</sub></sub>) = 0



$$
\left(\begin{array}{cc}
1 & 0 & 0 & 0 & 0 & 0\\
0 & 1 & 0 & 0 & 0 & 0\\
0 & 0 & 1 & 0 & 0 & 0\\
1 & 0 & 0 & 0 & 0 & 0\\
0 & 1 & 0 & 0 & 0 & 0\\
0 & 0 & 1 & 0 & 0 & 0\\
\end{array}\right)
\left(\begin{array}{cc}
prx\\
pry\\
prz\\
vrx\\
vry\\
vrz
\end{array}\right)
=
\left(\begin{array}{cc}
0\\
0\\
0\\
0\\
0\\
0\\
\end{array}\right)
$$ 