A = Button A

B = Button B

P = Price

---

A<sub>x</sub> · a + B<sub>x</sub> · b = P<sub>x</sub>

A<sub>y</sub> · a + B<sub>y</sub> · b = P<sub>y</sub>

---

a = (P<sub>x</sub> - B<sub>x</sub> · b) / A<sub>x</sub>

a = (P<sub>y</sub> - B<sub>y</sub> · b) / A<sub>y</sub>

---

a = (P<sub>x</sub> - B<sub>x</sub> · b) / A<sub>x</sub>

(P<sub>x</sub> - B<sub>x</sub> · b) / A<sub>x</sub> = (P<sub>y</sub> - B<sub>y</sub> · b) / A<sub>y</sub>

---

a = (P<sub>x</sub> - B<sub>x</sub> · b) / A<sub>x</sub>

A<sub>y</sub> · (P<sub>x</sub> - B<sub>x</sub> · b) = A<sub>x</sub> · (P<sub>y</sub> - B<sub>y</sub> · b)

---

a = (P<sub>x</sub> - B<sub>x</sub> · b) / A<sub>x</sub>

A<sub>y</sub> · P<sub>x</sub> - A<sub>y</sub> · B<sub>x</sub> · b = A<sub>x</sub> · P<sub>y</sub> - A<sub>x</sub> · B<sub>y</sub> · b

---

a = (P<sub>x</sub> - B<sub>x</sub> · b) / A<sub>x</sub>

A<sub>x</sub> · B<sub>y</sub> · b - A<sub>y</sub> · B<sub>x</sub> · b = A<sub>x</sub> · P<sub>y</sub> - A<sub>y</sub> · P<sub>x</sub>

---

a = (P<sub>x</sub> - B<sub>x</sub> · b) / A<sub>x</sub>

b · (A<sub>x</sub> · B<sub>y</sub> - A<sub>y</sub> · B<sub>x</sub>) = A<sub>x</sub> · P<sub>y</sub> - A<sub>y</sub> · P<sub>x</sub>

---

a = (P<sub>x</sub> - B<sub>x</sub> · b) / A<sub>x</sub>

b = (A<sub>x</sub> · P<sub>y</sub> - A<sub>y</sub> · P<sub>x</sub>) / (A<sub>x</sub> · B<sub>y</sub> - A<sub>y</sub> · B<sub>x</sub>)

---

A = (94,34)
B = (22,67)
P = (8400,5400)

---

b = (94 · 5400 - 34 · 8400) / (94 · 67 - 34 · 22)

a = (8400 - 22 · b) / 94

---

b = 40

a = (8400 - 22 · 40) / 94 = 80